SmallStep.v
@@ -2,23 +2,22 @@
 (* Licensing information is available in the LICENSE file. *)
 (* (C) 2020 Nandor Licker. All rights reserved. *)
 
+Require Import Coq.Lists.List.
+Require Import Coq.ZArith.ZArith.
 Require Import Values.
-Require Import LLIR.
 Require Import State.
 Require Import Maps.
-Require Import Coq.Lists.List.
+Require Import LLIR.LLIR.
+Require Import LLIR.Dom.
+Require Import LLIR.Eval.
 
 Import ListNotations.
 
-Inductive trace: Type.
 
-Inductive frame: Type :=
-  | Frame:
-    forall
-      (f: func)
-      (ret_pc: node)
-      (vregs: PTrie.t value),
-        frame.
+
+Inductive event: Type.
+
+Definition trace := list event.
 
 Definition stk_state := list frame.
 
@@ -33,9 +32,13 @@ Inductive state: Type :=
         state
   .
 
-Definition get_inst (stk: stk_state) (pc: node): option inst :=
+Definition get_inst (p: prog) (stk: stk_state) (pc: node): option inst :=
   match stk with
-  | (Frame f _ _) :: _ => f.(fn_insts) ! pc
+  | f :: _ =>
+    match p ! (f.(fr_func)) with
+    | Some func => func.(fn_insts) ! pc
+    | None => None
+    end
   | _ => None
   end.
 
@@ -51,14 +54,15 @@ Axiom eval_unop: ty -> unop -> value -> option value.
 
 Axiom eval_binop: ty -> binop -> value -> value -> option value.
 
-Inductive step: state -> trace -> state -> Prop :=
+Inductive step (p: prog): state -> trace -> state -> Prop :=
   | eval_jmp:
     forall
       (stk: stk_state) (mem: mem_state) (tr: trace)
       (pc: node)
       (target: node),
-      get_inst stk pc = Some (LLJmp target) ->
+      get_inst p stk pc = Some (LLJmp target) ->
       step
+        p
         (State stk mem pc)
         tr
         (State stk mem target)
@@ -68,10 +72,11 @@ Inductive step: state -> trace -> state -> Prop :=
       (pc: node)
       (cond: reg) (brancht: node) (branchf: node)
       (v: value),
-      get_inst stk pc = Some (LLJcc cond brancht branchf) ->
+      get_inst p stk pc = Some (LLJcc cond brancht branchf) ->
       get_vreg stk cond = Some v ->
       is_true v ->
       step
+        p
         (State stk mem pc)
         tr
         (State stk mem brancht)
@@ -81,10 +86,11 @@ Inductive step: state -> trace -> state -> Prop :=
       (pc: node)
       (cond: reg) (brancht: node) (branchf: node)
       (v: value),
-      get_inst stk pc = Some (LLJcc cond brancht branchf) ->
+      get_inst p stk pc = Some (LLJcc cond brancht branchf) ->
       get_vreg stk cond = Some v ->
       is_false v ->
       step
+        p
         (State stk mem pc)
         tr
         (State stk mem brancht)
@@ -95,11 +101,12 @@ Inductive step: state -> trace -> state -> Prop :=
       (ty: ty) (op: unop) (arg: reg) (dst: reg) (next: node)
       (arg_value: value) (dst_value: value)
       (stk': stk_state),
-      get_inst stk pc = Some (LLUnop (ty, dst) next op arg) ->
+      get_inst p stk pc = Some (LLUnop (ty, dst) next op arg) ->
       get_vreg stk arg = Some arg_value ->
       eval_unop ty op arg_value = Some dst_value ->
       set_vreg stk dst dst_value = Some stk' ->
       step
+        p
         (State stk mem pc)
         tr
         (State stk' mem next)
@@ -110,31 +117,67 @@ Inductive step: state -> trace -> state -> Prop :=
       (ty: ty) (op: binop) (lhs: reg) (rhs: reg) (dst: reg) (next: node)
       (lhs_value: value) (rhs_value: value) (dst_value: value)
       (stk': stk_state),
-      get_inst stk pc = Some (LLBinop (ty, dst) next op lhs rhs) ->
+      get_inst p stk pc = Some (LLBinop (ty, dst) next op lhs rhs) ->
       get_vreg stk lhs = Some lhs_value ->
       get_vreg stk rhs = Some rhs_value ->
       eval_binop ty op lhs_value rhs_value = Some dst_value ->
       set_vreg stk dst dst_value = Some stk' ->
       step
+        p
         (State stk mem pc)
         tr
         (State stk' mem next)
   .
 
-  (*
-  | LLConst (value: qword) (dst: reg) (next: node)
+Inductive star (p: prog): state -> trace -> state -> Prop :=
+  | star_refl:
+    forall (st: state),
+      star p st [] st
+  | star_step:
+    forall 
+      (st0: state) (st1: state) (st2: state)
+      (tr0: trace) (tr1: trace) (tr: trace)
+      (STAR: star p st0 tr0 st1)
+      (STEP: step p st1 tr1 st2),
+      star p st0 (tr0 ++ tr1) st2
+  .
 
-  | LLLd (addr: reg) (dst: reg) (next: node)
-  | LLSt (addr: reg) (val: reg) (next: node)
+(*
+Inductive ExecutionAt (p: prog): stk_state -> mem_state -> func -> node -> Prop :=
+  | exec_at:
+    forall 
+      (id: positive) (ret_pc: node) (pc: node) (vregs: PTrie.t value) 
+      (frs: list frame) (mem: mem_state) (f: func)
+      (FUNC: Some f = p ! id)
+      (INST: None <> f.(fn_insts) ! pc)
+      (r: reg),
+      ExecutionAt 
+        p
+        (Frame id ret_pc vregs :: frs) 
+        mem 
+        f
+        pc.
 
-  | LLArg (index: positive) (dst: reg) (next: node)
-
-  | LLFrame (object: positive) (dst: reg) (next: node)
-  | LLGlobal (object: positive) (dst: reg) (next: node)
-  | LLExtern (id: positive) (next: node)
-
-  | LLCall (callee: reg) (args: list reg) (dst: reg) (next: node)
-  | LLInvoke (callee: reg) (args: list reg) (dst: reg) (next: node) (exn: node)
-
-  | LLRet (value: reg)
-  *)
+Theorem exec_bb:
+  forall (p: prog)
+    (stk: stk_state) (mem: mem_state) (f: func) (h: node) (n: node),
+    ExecutionAt p stk mem f h ->
+    BasicBlock f h n ->
+    exists (stk': stk_state) (mem': mem_state) (tr: trace),
+      star p (State stk mem h) tr (State stk' mem' n).
+Proof.
+  intros p stk mem f h n Hexec Hbb.
+  induction Hbb.
+  { exists stk. exists mem. exists []. apply star_refl. }
+  {
+    destruct ((fn_insts f) ! elem) as [inst|] eqn:Hinst; try contradiction.
+    apply IHHbb in Hexec. clear IHHbb.
+    destruct Hexec as [stk' [mem' [tr Hstart]]].
+    clear INST.
+    destruct inst.
+    {
+      
+    }
+  }
+Qed.
+*)
