Typing.v
@@ -13,237 +13,217 @@ Require Import LLIR.Values.
 
 Definition type_env := PTrie.t ty.
 
+Definition ptr_ty := TInt I64.
+Definition syscall_ty := TInt I64.
 
+(* Returns the register defined by an instruction and its type. *)
+Definition get_inst_def (i: inst): option (ty * reg) :=
+  match i with
+  | LLSyscall dst _ _ _ => Some (syscall_ty, dst)
+  | LLCall dst _ _ _ => dst
+  | LLTCall _ _ => None
+  | LLInvoke dst _ _ _ _ => dst
+  | LLTInvoke _ _ _ => None
 
-(* Interface containing all target-specific information. *)
-Module Type ArchTy.
-  Parameter ptr_ty: ty.
-  Parameter syscall_ty: ty.
-End ArchTy.
+  | LLArg dst _ _ => Some dst
+  | LLInt8 dst _ _ => Some (TInt I8, dst)
+  | LLInt16 dst _ _ => Some (TInt I16, dst)
+  | LLInt32 dst _ _ => Some (TInt I32, dst)
+  | LLInt64 dst _ _ => Some (TInt I64, dst)
+  | LLMov dst _ _ => Some dst
 
-(* X86-specific typing. *)
-Module X86_ArchTy <: ArchTy.
-  Definition ptr_ty := TInt I64.
-  Definition syscall_ty := TInt I64.
-End X86_ArchTy.
+  | LLFrame dst _ _ _ => Some (ptr_ty, dst)
+  | LLGlobal dst _ _ _ => Some (ptr_ty, dst)
 
-(* Generic typing rules *)
-Module Type Typing.
-  Parameter ptr_ty: ty.
-  Parameter ty_env: func -> type_env.
-End Typing.
+  | LLLd dst _ _ => Some dst
+  | LLUndef dst _ => Some dst
+  | LLUnop dst _ _ _ => Some dst
+  | LLBinop dst _ _ _ _ => Some dst
+  | LLSelect dst _ _ _ _ => Some dst
 
-(* LLIR typing rules *)
-Module Target_Typing (ARCH: ArchTy) <: Typing.
-  Include ARCH.
+  | LLSt _ _ _ => None
+  | LLRet _ => None
+  | LLJcc _ _ _ => None
+  | LLJmp _ => None
+  | LLTrap => None
+  end.
 
-  (* Returns the register defined by an instruction and its type. *)
-  Definition get_inst_def (i: inst): option (ty * reg) :=
-    match i with
-    | LLSyscall dst _ _ _ => Some (ARCH.syscall_ty, dst)
-    | LLCall dst _ _ _ => dst
-    | LLTCall _ _ => None
-    | LLInvoke dst _ _ _ _ => dst
-    | LLTInvoke _ _ _ => None
+(* Type environment from instructions. *)
+Definition ty_env_inst (insts: inst_map): type_env :=
+  PTrie.fold
+    (fun env _ i =>
+      match get_inst_def i with
+      | Some (ty, dst) => PTrie.set env dst ty
+      | None => env
+      end)
+    insts PTrie.empty.
 
-    | LLArg dst _ _ => Some dst
-    | LLInt8 dst _ _ => Some (TInt I8, dst)
-    | LLInt16 dst _ _ => Some (TInt I16, dst)
-    | LLInt32 dst _ _ => Some (TInt I32, dst)
-    | LLInt64 dst _ _ => Some (TInt I64, dst)
-    | LLMov dst _ _ => Some dst
+(* Type environment from phis. *)
+Definition ty_env_phi (phis: phi_map): type_env :=
+  PTrie.fold
+    (fun env _ block =>
+      List.fold_left
+        (fun env p =>
+          match p with
+          | LLPhi (ty, dst) _ => PTrie.set env dst ty
+          end)
+        block env)
+    phis PTrie.empty.
 
-    | LLFrame dst _ _ _ => Some (ARCH.ptr_ty, dst)
-    | LLGlobal dst _ _ _ => Some (ARCH.ptr_ty, dst)
+(* Type environment for all registers. *)
+Definition ty_env (f: func): type_env :=
+  PTrie.union (ty_env_inst f.(fn_insts)) (ty_env_phi f.(fn_phis)).
 
-    | LLLd dst _ _ => Some dst
-    | LLUndef dst _ => Some dst
-    | LLUnop dst _ _ _ => Some dst
-    | LLBinop dst _ _ _ _ => Some dst
-    | LLSelect dst _ _ _ _ => Some dst
+(* Holds if the evironment has the correct type for a reg. *)
+Definition well_typed_reg (env: type_env) (r: reg) (t: ty) :=
+  env ! r = Some t.
 
-    | LLSt _ _ _ => None
-    | LLRet _ => None
-    | LLJcc _ _ _ => None
-    | LLJmp _ => None
-    | LLTrap => None
-    end.
+(* Typing rules for binary instructions. *)
+Inductive well_typed_binop: binop -> ty -> ty -> ty -> Prop :=
+  | type_cmp:
+    forall (t: ty) (dt: ty),
+      well_typed_binop LLCmp t t dt
+  | type_add:
+    forall (t: ty),
+      well_typed_binop LLAdd t t t
+  | type_sll:
+    forall (tl: ty_int) (tr: ty_int),
+      well_typed_binop LLSll (TInt tl) (TInt tr) (TInt tl)
+  .
 
-  (* Type environment from instructions. *)
-  Definition ty_env_inst (insts: inst_map): type_env :=
-    PTrie.fold
-      (fun env _ i =>
-        match get_inst_def i with
-        | Some (ty, dst) => PTrie.set env dst ty
-        | None => env
-        end)
-      insts PTrie.empty.
+(* Typing rules for unary instructions. *)
+Inductive well_typed_unop: unop -> ty -> ty -> Prop :=
+  | type_sext_i32_i64: well_typed_unop LLSext (TInt I32) (TInt I64)
+  .
 
-  (* Type environment from phis. *)
-  Definition ty_env_phi (phis: phi_map): type_env :=
-    PTrie.fold
-      (fun env _ block =>
-        List.fold_left
-          (fun env p =>
-            match p with
-            | LLPhi (ty, dst) _ => PTrie.set env dst ty
-            end)
-          block env)
-      phis PTrie.empty.
+(* Typing rules for instructions. *)
+Inductive well_typed_inst: type_env -> inst -> Prop :=
+  | type_jmp:
+    forall (env: type_env) (target: node),
+      well_typed_inst env (LLJmp target)
+  | type_jcc:
+    forall (env: type_env) (cond: reg) (bt: node) (bf: node) (i: ty_int)
+      (COND_TY: well_typed_reg env cond (TInt i)),
+      well_typed_inst env (LLJcc cond bt bf)
+  | type_ret:
+    forall (env: type_env) (ret: reg) (t: ty)
+      (RET_TY: well_typed_reg env ret t),
+      well_typed_inst env (LLRet (Some ret))
+  | type_ret_void:
+    forall (env: type_env),
+      well_typed_inst env (LLRet None)
+  | type_st:
+    forall (env: type_env) (next: node) (addr: reg) (val: reg) (t: ty)
+      (ADDR_TY: well_typed_reg env addr ptr_ty)
+      (VAL_TY: well_typed_reg env val t),
+      well_typed_inst env (LLSt next addr val)
+  | type_undef:
+    forall (env: type_env) (next: node) (dst: reg) (t: ty)
+      (DST_TY: well_typed_reg env dst t),
+      well_typed_inst env (LLUndef (t, dst) next)
+  | type_ld:
+    forall (env: type_env) (next: node) (dst: reg) (t: ty) (addr: reg)
+      (ADDR_TY: well_typed_reg env addr ptr_ty)
+      (DST_TY: well_typed_reg env dst t),
+      well_typed_inst env (LLLd (t, dst) next addr)
+  | type_frame:
+    forall (env: type_env) (dst:reg) (next: node) (object: positive) (offset: nat)
+      (DST_TY: well_typed_reg env dst ptr_ty),
+      well_typed_inst env (LLFrame dst next object offset)
+  | type_global:
+    forall (env: type_env) (dst: reg) (next: node) (object: positive) (offset: nat)
+      (DST_TY: well_typed_reg env dst ptr_ty),
+      well_typed_inst env (LLGlobal dst next object offset)
+  | type_int8:
+    forall (env: type_env) (dst: reg) (next: node) (val: INT8.t)
+      (DST_TY: well_typed_reg env dst (TInt I8)),
+      well_typed_inst env (LLInt8 dst next val)
+  | type_int16:
+    forall (env: type_env) (dst: reg) (next: node) (val: INT16.t)
+      (DST_TY: well_typed_reg env dst (TInt I16)),
+      well_typed_inst env (LLInt16 dst next val)
+  | type_int32:
+    forall (env: type_env) (dst: reg) (next: node) (val: INT32.t)
+      (DST_TY: well_typed_reg env dst (TInt I32)),
+      well_typed_inst env (LLInt32 dst next val)
+  | type_int64:
+    forall (env: type_env) (dst: reg) (next: node) (val: INT64.t)
+      (DST_TY: well_typed_reg env dst (TInt I64)),
+      well_typed_inst env (LLInt64 dst next val)
+  | type_arg:
+    forall (env: type_env) (t: ty) (dst: reg) (next: node) (idx: nat)
+      (DST_TY: well_typed_reg env dst t),
+      well_typed_inst env (LLArg (t, dst) next idx)
+  | type_binop:
+    forall (env: type_env) (op: binop) (next: node)
+      (l: reg) (tl: ty) (r: reg) (tr: ty) (dst: reg) (t: ty)
+      (LHS_TY: well_typed_reg env l tl)
+      (RHS_TY: well_typed_reg env r tr)
+      (DST_TY: well_typed_reg env dst t)
+      (OP: well_typed_binop op tl tr t),
+      well_typed_inst env (LLBinop (t, dst) next op l r)
+  | type_unop:
+    forall (env: type_env) (op: unop) (next: node)
+      (arg: reg) (argt: ty) (dst: reg) (t: ty)
+      (ARG_TY: well_typed_reg env arg argt)
+      (DST_TY: well_typed_reg env dst t)
+      (OP: well_typed_unop op argt t),
+      well_typed_inst env (LLUnop (t, dst) next op arg)
+  | type_invoke_void:
+    forall (env: type_env) (next: node)
+      (dst: reg) (t: ty)
+      (callee: reg) (args: list reg) (exn: node)
+      (CALLEE_TY: well_typed_reg env callee ptr_ty),
+      well_typed_inst env (LLInvoke (Some (t, dst)) next callee args exn)
+  | type_call_void:
+    forall (env: type_env) (next: node)
+      (callee: reg) (args: list reg)
+      (CALLEE_TY: well_typed_reg env callee ptr_ty),
+      well_typed_inst env (LLCall None next callee args)
+  | type_call:
+    forall (env: type_env) (next: node)
+      (callee: reg) (args: list reg) (dst: reg) (t: ty)
+      (CALLEE_TY: well_typed_reg env callee ptr_ty)
+      (DST_TY: well_typed_reg env dst t),
+      well_typed_inst env (LLCall (Some (t, dst)) next callee args)
+  | type_tcall:
+    forall (env: type_env)
+      (callee: reg) (args: list reg)
+      (CALLEE_TY: well_typed_reg env callee ptr_ty),
+      well_typed_inst env (LLTCall callee args)
+  | type_syscall:
+    forall (env: type_env) (next: node)
+      (sno: reg) (args: list reg) (tsno: ty_int) (dst: reg) (t: ty)
+      (SNO_TY: well_typed_reg env sno (TInt tsno))
+      (DST_TY: well_typed_reg env dst t),
+      well_typed_inst env (LLSyscall dst next sno args)
+  | type_trap:
+    forall (env: type_env),
+      well_typed_inst env LLTrap
+  .
 
-  (* Type environment for all registers. *)
-  Definition ty_env (f: func): type_env :=
-    PTrie.union (ty_env_inst f.(fn_insts)) (ty_env_phi f.(fn_phis)).
+Definition well_typed_insts (env: type_env) (insts: inst_map) :=
+  forall (n: node) (i: inst),
+    Some i = insts ! n -> well_typed_inst env i.
 
-  (* Holds if the evironment has the correct type for a reg. *)
-  Definition well_typed_reg (env: type_env) (r: reg) (t: ty) :=
-    env ! r = Some t.
+Inductive well_typed_phi: type_env -> phi -> Prop :=
+  | typed_phi:
+    forall (env: type_env) (dst: reg) (t: ty) (ins: list (node * reg))
+      (INS: forall (n: node) (r: reg), In (n, r) ins -> well_typed_reg env r t),
+      well_typed_phi env (LLPhi (t, dst) ins)
+  .
 
-  (* Typing rules for binary instructions. *)
-  Inductive well_typed_binop: binop -> ty -> ty -> ty -> Prop :=
-    | type_cmp:
-      forall (t: ty) (dt: ty),
-        well_typed_binop LLCmp t t dt
-    | type_add:
-      forall (t: ty),
-        well_typed_binop LLAdd t t t
-    | type_sll:
-      forall (tl: ty_int) (tr: ty_int),
-        well_typed_binop LLSll (TInt tl) (TInt tr) (TInt tl)
-    .
+Definition well_typed_phis (env: type_env) (phis: phi_map) :=
+  forall (n: node) (block: list phi) (p: phi),
+    Some block = phis ! n ->
+    In p block ->
+    well_typed_phi env p.
 
-  (* Typing rules for unary instructions. *)
-  Inductive well_typed_unop: unop -> ty -> ty -> Prop :=
-    | type_sext_i32_i64: well_typed_unop LLSext (TInt I32) (TInt I64)
-    .
+Definition well_typed_func (f: func) :=
+  well_typed_insts (ty_env f) f.(fn_insts)
+  /\
+  well_typed_phis (ty_env f) f.(fn_phis).
 
-  (* Typing rules for instructions. *)
-  Inductive well_typed_inst: type_env -> inst -> Prop :=
-    | type_jmp:
-      forall (env: type_env) (target: node),
-        well_typed_inst env (LLJmp target)
-    | type_jcc:
-      forall (env: type_env) (cond: reg) (bt: node) (bf: node) (i: ty_int)
-        (COND_TY: well_typed_reg env cond (TInt i)),
-        well_typed_inst env (LLJcc cond bt bf)
-    | type_ret:
-      forall (env: type_env) (ret: reg) (t: ty)
-        (RET_TY: well_typed_reg env ret t),
-        well_typed_inst env (LLRet (Some ret))
-    | type_ret_void:
-      forall (env: type_env),
-        well_typed_inst env (LLRet None)
-    | type_st:
-      forall (env: type_env) (next: node) (addr: reg) (val: reg) (t: ty)
-        (ADDR_TY: well_typed_reg env addr ARCH.ptr_ty)
-        (VAL_TY: well_typed_reg env val t),
-        well_typed_inst env (LLSt next addr val)
-    | type_undef:
-      forall (env: type_env) (next: node) (dst: reg) (t: ty)
-        (DST_TY: well_typed_reg env dst t),
-        well_typed_inst env (LLUndef (t, dst) next)
-    | type_ld:
-      forall (env: type_env) (next: node) (dst: reg) (t: ty) (addr: reg)
-        (ADDR_TY: well_typed_reg env addr ARCH.ptr_ty)
-        (DST_TY: well_typed_reg env dst t),
-        well_typed_inst env (LLLd (t, dst) next addr)
-    | type_frame:
-      forall (env: type_env) (dst:reg) (next: node) (object: positive) (offset: nat)
-        (DST_TY: well_typed_reg env dst ARCH.ptr_ty),
-        well_typed_inst env (LLFrame dst next object offset)
-    | type_global:
-      forall (env: type_env) (dst: reg) (next: node) (object: positive) (offset: nat)
-        (DST_TY: well_typed_reg env dst ARCH.ptr_ty),
-        well_typed_inst env (LLGlobal dst next object offset)
-    | type_int8:
-      forall (env: type_env) (dst: reg) (next: node) (val: INT8.t)
-        (DST_TY: well_typed_reg env dst (TInt I8)),
-        well_typed_inst env (LLInt8 dst next val)
-    | type_int16:
-      forall (env: type_env) (dst: reg) (next: node) (val: INT16.t)
-        (DST_TY: well_typed_reg env dst (TInt I16)),
-        well_typed_inst env (LLInt16 dst next val)
-    | type_int32:
-      forall (env: type_env) (dst: reg) (next: node) (val: INT32.t)
-        (DST_TY: well_typed_reg env dst (TInt I32)),
-        well_typed_inst env (LLInt32 dst next val)
-    | type_int64:
-      forall (env: type_env) (dst: reg) (next: node) (val: INT64.t)
-        (DST_TY: well_typed_reg env dst (TInt I64)),
-        well_typed_inst env (LLInt64 dst next val)
-    | type_arg:
-      forall (env: type_env) (t: ty) (dst: reg) (next: node) (idx: nat)
-        (DST_TY: well_typed_reg env dst t),
-        well_typed_inst env (LLArg (t, dst) next idx)
-    | type_binop:
-      forall (env: type_env) (op: binop) (next: node)
-        (l: reg) (tl: ty) (r: reg) (tr: ty) (dst: reg) (t: ty)
-        (LHS_TY: well_typed_reg env l tl)
-        (RHS_TY: well_typed_reg env r tr)
-        (DST_TY: well_typed_reg env dst t)
-        (OP: well_typed_binop op tl tr t),
-        well_typed_inst env (LLBinop (t, dst) next op l r)
-    | type_unop:
-      forall (env: type_env) (op: unop) (next: node)
-        (arg: reg) (argt: ty) (dst: reg) (t: ty)
-        (ARG_TY: well_typed_reg env arg argt)
-        (DST_TY: well_typed_reg env dst t)
-        (OP: well_typed_unop op argt t),
-        well_typed_inst env (LLUnop (t, dst) next op arg)
-    | type_invoke_void:
-      forall (env: type_env) (next: node)
-        (dst: reg) (t: ty)
-        (callee: reg) (args: list reg) (exn: node)
-        (CALLEE_TY: well_typed_reg env callee ARCH.ptr_ty),
-        well_typed_inst env (LLInvoke (Some (t, dst)) next callee args exn)
-    | type_call_void:
-      forall (env: type_env) (next: node)
-        (callee: reg) (args: list reg)
-        (CALLEE_TY: well_typed_reg env callee ARCH.ptr_ty),
-        well_typed_inst env (LLCall None next callee args)
-    | type_call:
-      forall (env: type_env) (next: node)
-        (callee: reg) (args: list reg) (dst: reg) (t: ty)
-        (CALLEE_TY: well_typed_reg env callee ARCH.ptr_ty)
-        (DST_TY: well_typed_reg env dst t),
-        well_typed_inst env (LLCall (Some (t, dst)) next callee args)
-    | type_tcall:
-      forall (env: type_env)
-        (callee: reg) (args: list reg)
-        (CALLEE_TY: well_typed_reg env callee ARCH.ptr_ty),
-        well_typed_inst env (LLTCall callee args)
-    | type_syscall:
-      forall (env: type_env) (next: node)
-        (sno: reg) (args: list reg) (tsno: ty_int) (dst: reg) (t: ty)
-        (SNO_TY: well_typed_reg env sno (TInt tsno))
-        (DST_TY: well_typed_reg env dst t),
-        well_typed_inst env (LLSyscall dst next sno args)
-    | type_trap:
-      forall (env: type_env),
-        well_typed_inst env LLTrap
-    .
-
-  Definition well_typed_insts (env: type_env) (insts: inst_map) :=
-    forall (n: node) (i: inst),
-      Some i = insts ! n -> well_typed_inst env i.
-
-  Inductive well_typed_phi: type_env -> phi -> Prop :=
-    | typed_phi:
-      forall (env: type_env) (dst: reg) (t: ty) (ins: list (node * reg))
-        (INS: forall (n: node) (r: reg), In (n, r) ins -> well_typed_reg env r t),
-        well_typed_phi env (LLPhi (t, dst) ins)
-    .
-
-  Definition well_typed_phis (env: type_env) (phis: phi_map) :=
-    forall (n: node) (block: list phi) (p: phi),
-      Some block = phis ! n ->
-      In p block ->
-      well_typed_phi env p.
-
-  Definition well_typed (f: func) :=
-    well_typed_insts (ty_env f) f.(fn_insts)
-    /\
-    well_typed_phis (ty_env f) f.(fn_phis).
-End Target_Typing.
-
-Module X86_Typing := Target_Typing (X86_ArchTy).
+Definition well_typed_prog (p: prog) :=
+  forall (n: name) (f: func),
+    Some f = p ! n -> well_typed_func f.
